theories/interop/wrapper_wp_boundary_laws.v
@@ -40,37 +40,37 @@ Lemma wrap_interp_c_to_ml w ρc mem θ v lv (X : val → wrapstateML → store �
   at_boundary _.
 Proof.
   iIntros (Hlv Hc_to_ml) "Hσ HGC Hnb #Hblk".
-  iNamed "Hσ". iNamed "SIC". iNamed "HGC". simplify_eq.
+  iNamed "Hσ". iNamed "SIC". iNamed "HGC". simplify_eq. SI_GC_agree.
 
-  iAssert (⌜is_val χvirt (ζσ ∪ ζrest) v lv⌝)%I as "%Hval".
-  by iApply (block_sim_to_ghost_state with "HAχvirt HAζrest [] [] [] [] Hblk").
-  iAssert (⌜∀ k lv, roots_m !! k = Some lv → ∃ w, mem !! k = Some (Storing w) ∧ repr_lval θ lv w⌝)%I as "%Hroots".
+  iAssert (⌜is_val χvirt (ζσ ∪ ζvirt) v lv⌝)%I as "%Hval".
+  by iApply (block_sim_to_ghost_state with "GCχvirt GCζvirt [] [] [] [] Hblk").
+  iAssert (⌜∀ k lv, roots_m !! k = Some lv →
+            ∃ w, mem !! k = Some (Storing w) ∧ repr_lval (θC ρc) lv w⌝)%I as "%Hroots".
   1: { iIntros (kk vv Hroots).
-       iPoseProof (big_sepM_lookup with "Hrootspto") as "(%wr & Hwr & %Hw2)"; first done.
+       iPoseProof (big_sepM_lookup with "GCrootspto") as "(%wr & Hwr & %Hw2)"; first done.
        iExists wr. iSplit; last done. iApply (gen_heap_valid with "HσC Hwr"). }
   apply map_Forall_lookup_2 in Hroots.
-  iPoseProof (ghost_var_agree with "HAGCθ HAθ") as "%Hagree1"; subst θ.
-  iPoseProof (ghost_var_agree with "HArootss HAroots") as "%Hagree2".
-  iMod (ghost_var_update_halves with "Hnb [HAGCbound HAbound]") as "(Hb & Hbound)".
+  iMod (ghost_var_update_halves with "Hnb [GCbound SIbound]") as "(Hb & SIbound)".
   (* Coq fails to infer ghost_var_fractional in time *)
-  1: iPoseProof (@fractional.fractional_merge _ _ _ _ _ _ (ghost_var_fractional _ _) with "HAGCbound HAbound") as "HH".
+  1: iPoseProof (@fractional.fractional_merge _ _ _ _ _ _ (ghost_var_fractional _ _)
+         with "GCbound SIbound") as "HH".
   1: by assert ((1 / 4 + 1 / 4 = 1 / 2)%Qp) as -> by compute_done.
   destruct (make_repr (θC ρc) roots_m mem) as [privmem Hpriv]; try done.
-  iMod (ghost_var_update_halves with "HAGCθ HAθ") as "(HAGCθ & HAθ)".
-  iMod (set_to_none with "HσC Hrootspto") as "(HσC & Hrootspto)"; first done.
+  iMod (ghost_var_update_halves with "GCζ SIζ") as "(GCζ & SIζ)".
+  iMod (ghost_var_update_halves with "GCχ SIχ") as "(GCχ & SIχ)".
+  iMod (ghost_var_update_halves with "GCθ SIθ") as "(GCθ & SIθ)".
+  iMod (ghost_var_update_halves with "GCroots SIroots") as "(GCroots & SIroots)".
+  iMod (set_to_none with "HσC GCrootspto") as "(HσC & GCrootspto)"; first done.
 
   iModIntro. iExists _, _. iSplit.
-  { iPureIntro. eapply (Hc_to_ml σMLvirt _ _ (ζσ ∪ ζrest) ζσ χvirt ζrest roots_m privmem).
+  { iPureIntro. eapply (Hc_to_ml σMLvirt _ _ (ζσ ∪ ζvirt) ζσ χvirt ζvirt roots_m privmem).
     all: try done. by rewrite map_union_comm. }
-  iSplitR "Hbound"; last by iFrame "Hbound".
+  iSplitR "SIbound"; last by iFrame "SIbound".
   rewrite /= /named.
-  iSplitL "HAσMLv HAnMLv HAσdom".
+  iSplitL "GCσMLv GCnMLv GCσdom".
   { iExists nMLv; iFrame. }
   unfold private_state_interp, ML_state_interp, GC_token_remnant, named; cbn.
-  iFrame. iSplitL "HnC"; first by iExists _.
-  rewrite <- Hagree2.
-  iFrame "HAroots".
-  iPureIntro; split_and!.
+  iExists _. iFrame. iPureIntro; split_and!.
   1: destruct Hχvirt as (_ & HHH); apply HHH.
   1: apply Hother_blocks.
   1: destruct Hpriv as (mem_r & ->%repr_roots_dom & Hpriv2 & Hpriv3); by apply map_disjoint_dom.
@@ -87,38 +87,43 @@ Lemma wrap_interp_ml_to_c vs ρml σ ws ρc mem :
   (∃ lvs, block_sim_arr vs lvs ∗ ⌜Forall2 (repr_lval (θC ρc)) lvs ws⌝).
 Proof.
   iIntros (Hml_to_c) "Hst Hb".
-  iNamed "Hst". iNamed "SIML". iNamed "HAGCrem".
+  iNamed "Hst". iNamed "SIML". iNamed "SIGCrem".
   destruct Hml_to_c as (ζσ & ζnewimm & lvs & HH).
   destruct HH as (Hmono & Hblocks & Hprivblocks & HζC & Hζdisj &
                     Hstore & Hvals & ? & ? & ? & Hroots & ?).
 
-  iMod (ghost_var_update_halves with "Hb HAbound") as "(Hnb & Hnb2)".
+  iMod (ghost_var_update_halves with "Hb SIbound") as "(Hnb & Hnb2)".
   1: iPoseProof (@fractional.fractional _ _ (ghost_var_fractional _ _)) as "[HH _]".
-  iDestruct ("HH" with "[Hnb2]") as "(HAGCbound & HAbound)".
+  iDestruct ("HH" with "[Hnb2]") as "(GCbound & SIbound)".
   1: by assert ((1 / 4 + 1 / 4 = 1 / 2)%Qp) as <- by compute_done.
   iClear "HH".
-  iMod (ghost_var_update_halves with "HAθ HAGCθ") as "(HAθ & HAGCθ)".
+  iMod (ghost_var_update_halves with "SIζ GCζ") as "(SIζ & GCζ)".
+  iMod (ghost_var_update_halves with "SIχ GCχ") as "(SIχ & GCχ)".
+  iMod (ghost_var_update_halves with "SIθ GCθ") as "(SIθ & GCθ)".
+  iMod (ghost_var_update_halves with "SIroots GCroots") as "(SIroots & GCroots)".
   apply map_disjoint_union_r in Hζdisj as [Hζdisj1 Hζdisj2].
-  iMod (lstore_own_insert_many with "HAζrest") as "(HAζrest & Hζnewimm)"; first done.
-  iMod (lloc_own_mono with "HAχ") as "HAχ"; first done.
+  iMod (lstore_own_insert_many with "SIζvirt") as "(SIζvirt & SIζnewimm)"; first done.
+  iMod (lloc_own_mono with "SIAχ") as "SIAχ"; first done.
   assert (ζσ ##ₘ ζnewimm) as Hdisj2 by by eapply is_store_blocks_is_private_blocks_disjoint.
   assert (ζC ρc = ζσ ∪ (ζML ρml ∪ ζnewimm)) as H6B.
   1: { rewrite map_union_assoc. rewrite (map_union_comm ζσ); first done. by symmetry. }
-  iPoseProof (block_sim_arr_of_ghost_state _ _ _ _ _ vs lvs with "HAχ HAζrest [] [] [] [] []") as "#Hsim".
+  iPoseProof (block_sim_arr_of_ghost_state _ _ _ _ _ vs lvs with "SIAχ SIζvirt [] [] [] [] []") as "#Hsim".
   1-5: iPureIntro. 5: eassumption. 1-3:done. 1: by apply map_disjoint_union_r.
-  iMod (set_to_some with "HAσCv Hrootspto") as "(HAσCv & Hrootspto)"; first done.
+  iMod (set_to_some with "HσCv GCrootspto") as "(HσCv & GCrootspto)"; first done.
 
   iModIntro. iFrame "Hnb". rewrite /= /named.
-  iSplitR "HAGCθ HAGCbound HArootsm HArootss Hrootspto".
-  { iSplitL "HAσCv HAnCv". { iExists nCv. iFrame. }
-    rewrite /C_state_interp /= /named.
-    iExists (ζC ρc), ζσ, (ζML ρml ∪ ζnewimm), (χC ρc), σ. iFrame.
-    rewrite Hroots. iFrame "HAroots".
-    iSplitL "HvML"; first by iExists _.
-    rewrite pub_locs_in_lstore_insert_priv_store; last done.
-    erewrite pub_locs_in_lstore_mono at 1; [| eauto..]; [].
-    iFrame "HAχNone".
-    iPureIntro. split_and!; eauto.
+  iSplitL "HσCv HnCv SIζ SIχ SIθ SIroots SIbound".
+  { iSplitL "HσCv HnCv". by iExists _; iFrame.
+    rewrite /C_state_interp /named. iFrame. }
+  iSplit.
+  { rewrite /GC /named.
+    iExists (ζC ρc), (ζC ρc), ζσ, (ζML ρml ∪ ζnewimm).
+    iExists (χC ρc), (χC ρc), σ, (rootsC ρc), (rootsML ρml).
+    iExists _. iFrame. iSplit.
+    { rewrite pub_locs_in_lstore_insert_priv_store; last done.
+      erewrite pub_locs_in_lstore_mono at 1; [| eauto..]; [].
+      iFrame "SIAχNone". }
+    iPureIntro; split_and!; eauto.
     { reflexivity. }
     { by apply map_disjoint_union_r. }
     { rewrite dom_union_L. apply union_least.
@@ -128,9 +133,7 @@ Proof.
         by eapply elem_of_dom_2, Hprivblocks. }
     { split; first done. split; first apply Hmono.
       intros γ v1 v2 HH1 HH2. simplify_map_eq. econstructor. } }
-  { iSplitL; last by (iExists _; iFrame "Hsim").
-    rewrite /GC /named. iExists (dom (rootsML ρml)), (rootsML ρml).
-    iFrame. done. }
+  { iExists _; by iFrame "Hsim". }
 Qed.
 
 End BoundaryLaws.
